# 3.72

## Solution

Assembly code:

```asm
	long aframe(long n, long idx, long *q)
	n in %rdi, idx in %rsi, q in %rdx
1	aframe:
2	pushq	%rbp
3	movq	%rsp, %rbp
4	subq	$16, %rsp			Allocate space for i (%rsp = s1)
5	leaq	30(,%rdi,8), %rax
6	andq	$-16, %rax
7	subq	%rax, %rsp			Allocate space for array p (%rsp = s2)
8	leaq	15(%rsp), %r8
9	andq	$-16, %r8			Set %r8 to &p[0]
	â‹®
```

#### A.

$$
s2 = s1 - (30 + 8 \cdot n)\ \text{AND}\ (-16)
$$

The $k\ \text{AND}\ (-16)$ is equivalent to $k - k \bmod 16$ (from the bitwise representation
of -16)

We have,

$(30 + 8 \cdot n)\ \text{AND}\ (-16) = 30 + 8 \cdot n - (30 + 8 \cdot n) \bmod 16$

$= 30 + 8 \cdot n - (16 + 8 \cdot n + 8 + 6) \bmod 16$

$= 30 + 8 \cdot n - (16 + 8 \cdot (n+1) + 6) \bmod 16$

We have two cases, when n is even and when is odd

**When n is even,**

$n = 2k$

$\implies (16 + 8 \cdot (n + 1) + 6) \bmod 16 = (16 + 8 \cdot (2k + 1) + 6) \bmod 16$

$= (16 \cdot (k + 1) + 14) \bmod 16$

$= 14$

$(30 + 8 \cdot n)\ \text{AND}\ (-16) = 30 + 8 \cdot n - 14 = 16 + 8 \cdot n$

**When n is odd,**

n + 1 is even. $\implies n + 1 = 2k$

$(16 + 8 \cdot (n + 1) + 6) \bmod 16 = (16 + 8 \cdot (2k) + 6) \bmod 16$

$= 6$

We get, $(30 + 8 \cdot n)\ \text{AND}\ (-16) = 30 + 8 \cdot n - 6 = 24 + 8 \cdot n$

$$
\begin{align}
s_2 = \begin{cases} s_1 - 8 \cdot n - 16 & \text{if n is even} \\
s_1 - 8 \cdot n - 24 & \text{if n is odd} \end{cases}
\end{align}
$$

#### B.

From lines 8 and 9, $p = 15 + s_2\ \text{AND}\ (-16)$.

$= 15 + s_2 - (15 + s_2) \bmod 16$

$(15 + s_2) \bmod 16 = (15 \bmod 16 + s_2 \bmod 16) \bmod 16$

$= (15 + s_2 \bmod 16) \bmod 16$

$s_2 \bmod 16$ can have 16 values, from 0 to 15.

We have these two cases:

**Case 1:** $s_2 \bmod 16 = 0$

$(15 + s_2 \bmod 16) \bmod 16 = 15$, and we get $p = 15 + s_2 - 15 = s_2$

**Case 2:** $1 <= (s_2 \bmod 16) <= 15$

Let $k = s_2 \bmod 16$

$(15 + k) \bmod 16 = (16 - 1 + k) \bmod 16 = (k - 1) \bmod 16$

$0 <= k - 1 <= 14 \implies p = 15 + s_2 - (s_2 \bmod 16 - 1) = 16 + s_2 - s_2 \bmod 16$

$$
\begin{align}
p = \begin{cases} s_2 & \text{if $s_2$ is a multiple of 16} \\
s_2 + 16 - s_2 \bmod 16 & \text{otherwise} \end{cases}
\end{align}
$$

#### C.

$e_1 + e_2 = s_1 - s_2$

From A,

$e_1 + e_2$ is either 16 (when $n$ is even) or 24 (when $n$ is odd).

From B,

$e2$ is either 0 (when $s_2$, and consequently $s_1$, as the offset between $s_1$ and $s_2$
is also a multiple of 16), or $16 - s_2 mod 16$ (same as $16 - s_1 mod 16$).

We end up with four cases

$$
\begin{align}
e_1 = \begin{cases} 24 - 0 & \text{if $s_1$ is a multiple of 16 and n is odd} \\
24 - (16 - s_1 \bmod 16) & \text{if $s_1$ is not a multiple of 16 and n is odd} \\
16 - 0 & \text{if $s_1$ is a multiple of 16 and n is even} \\
16 - (16 - s_1 \bmod 16) & \text{if $s_1$ is not a mulitiple of 16 and n is even} \end{cases}
\end{align}
$$

By comparing these cases, the case for maximum is case 1 where $e_1$ is 24, and the case for minimum
is the last one, where $e_1$ is 1 when $s_1 \bmod 16$ is 1.

#### D.

Always a multiple of 16 relative to $s_1$.
